Fixes + many more things to fix later

ex/InitFreezeRef.fst
@@ -9,20 +9,19 @@ open FStar.ST
 
 open FStar.MRef
 
-(*
- * A reference that starts uninitialized (unreadble), can be written to (mutable), and then ultimately can be frozen
- *)
+(* * A reference that starts uninitialized (unreadble), can be written to
+     (mutable), and then ultimately can be frozen (can no longer change) *)
 
 (*
  * Three states that the refernce can be in
  *)
-private type rstate (a:Type) =
-  | Empty  : rstate a        //starts as Empty
+type rstate (a:Type) =
+  | Empty  : rstate a         //starts as Empty
   | Mutable: v:a -> rstate a  //becomes Mutable
   | Frozen : v:a -> rstate a  //frozen ultimately
 
 (* Trying to define the state evolution as a preorder *)
-private let evolve_broken0 (a:Type) :relation (rstate a) =
+let evolve_broken' (a:Type) :relation (rstate a) =
   fun r1 r2 ->
   match r1, r2 with
   | Empty,      Mutable _
@@ -30,20 +29,26 @@ private let evolve_broken0 (a:Type) :relation (rstate a) =
   | Mutable v1, Frozen v2 -> v1 == v2
   | _, _ -> False
 
-(* private let evolve_broken (a:Type) :preorder (rstate a) = evolve_broken0 a
-   -- fails as it should *)
+[@expect_failure]
+let evolve_broken (a:Type) : Tot (preorder (rstate a)) = evolve_broken' a
 
-private let evolve (a:Type) :relation (rstate a) =
-  fun r1 r2 -> admit ()
+let evolve' (a:Type) :relation (rstate a) =
+  fun r1 r2 ->
+  match r1, r2 with
+  | Empty, _
+  | Mutable _, Mutable _
+  | Mutable _, Frozen _  -> True 
+  | Frozen v1, Frozen v2 -> v1 == v2
+  | _, _ -> False
+let evolve (a:Type) : Tot (preorder (rstate a)) = evolve' a
 
-(* Abstract type eref *)
-abstract type eref (a:Type) :Type0 = mref (rstate a) (evolve a)
+type eref (a:Type) :Type0 = mref (rstate a) (evolve a)
 
 (* Ghost addr_of function *)
-abstract let addr_of (#a:Type0) (r:eref a) :GTot nat = addr_of r
+let addr_of (#a:Type0) (r:eref a) :GTot nat = addr_of r
 
 (* Liveness of eref *)
-abstract let contains (#a:Type0) (h:heap) (r:eref a) :Type0 = h `Heap.contains` r
+let contains (#a:Type0) (h:heap) (r:eref a) :Type0 = h `Heap.contains` r
 
 (* Freshness predicate *)
 let fresh (#a:Type0) (r:eref a) (h0 h1:heap) :Type0 =
@@ -54,7 +59,7 @@ let fresh (#a:Type0) (r:eref a) (h0 h1:heap) :Type0 =
  * sel from an Empty reference returns None
  * But our high-level interface for reading reference should ensure that read cannot be called on Empty refs
  *)
-abstract let sel (#a:Type0) (h:heap) (r:eref a) :GTot (option a)
+let sel (#a:Type0) (h:heap) (r:eref a) :GTot (option a)
   = let x = sel h r in
     match x with
     | Empty     -> None
@@ -64,23 +69,23 @@ abstract let sel (#a:Type0) (h:heap) (r:eref a) :GTot (option a)
 (***** set up predicates *****)
 
 (* An eref is readable if it is not Empty *)
-private let readable_pred (#a:Type) :rstate a -> Type
+let readable_pred (#a:Type) :rstate a -> Type
   = fun x -> (~ (Empty? x))
 
 (* Clients can to play with readable predicate *)
-abstract let readable (#a:Type0) (r:eref a) :Type0
+let readable (#a:Type0) (r:eref a) :Type0
   = token r readable_pred
 
 (* Let's try to do the same for writable, a Frozen ref is non mutable *)
 private let writable_pred (#a:Type0) :rstate a -> Type
   = fun x -> Empty? x \/ Mutable? x
 
-(* abstract let writable (#a:Type0) (r:eref a) :Type0
+(* let writable (#a:Type0) (r:eref a) :Type0
   = token r (writable_pred #a)
   -- fails as it should, why? *)
 
 (* Mutability is a stateful invariant, note this is still abstract, our interface needs to take care of it *)
-abstract let writable_in (#a:Type0) (r:eref a) (h:heap) :Type0
+let writable_in (#a:Type0) (r:eref a) (h:heap) :Type0
   = let x = Heap.sel h r in Empty? x \/ Mutable? x
 
 (* Setup for frozen predicate *)
@@ -88,12 +93,12 @@ private let frozen_at_pred (#a:Type0) (x:a) :rstate a -> Type
   = fun y -> y == Frozen x
 
 (* frozen_at_pred is stable *)
-abstract let frozen_at (#a:Type0) (r:eref a) (x:a) :Type0
+let frozen_at (#a:Type0) (r:eref a) (x:a) :Type0
   = token r (frozen_at_pred x)
 
 (* fun begins *)
 
-abstract let alloc (a:Type0)
+let alloc (a:Type0)
   :ST (eref a) (requires (fun _       -> True))
                (ensures  (fun h0 r h1 ->
 	                  modifies !{} h0 h1 /\  //existing refs are unmodified
@@ -102,7 +107,7 @@ abstract let alloc (a:Type0)
 			  sel h1 r == None))    //sel returns None
   = admit ()
 
-abstract let write (#a:Type0) (r:eref a) (x:a)
+let write (#a:Type0) (r:eref a) (x:a)
   :ST unit (fun h0      -> r `writable_in` h0)  //stateful precondition that eref is mutable
            (fun h0 _ h1 -> modifies (Set.singleton (addr_of r)) h0 h1 /\  //only modify the addr of eref
 	                readable r                                 /\  //the eref now becomes (or remains) readale
@@ -110,13 +115,13 @@ abstract let write (#a:Type0) (r:eref a) (x:a)
 			sel h1 r == Some x)                            //sel returns what you wrote
   = admit ()
 
-abstract let read (#a:Type0) (r:eref a{readable r})  //note the precondition asks for readability of the eref
+let read (#a:Type0) (r:eref a{readable r})  //note the precondition asks for readability of the eref
   :ST a (requires (fun _       -> True))
         (ensures  (fun h0 x h1 -> h0 == h1 /\            //heap remains same
 	                       sel h1 r == Some x))  //return what sel returns
   = admit ()
 
-abstract let freeze (#a:Type0) (r:eref a{readable r})  //the precondition that we need is still readable
+let freeze (#a:Type0) (r:eref a{readable r})  //the precondition that we need is still readable
   :ST a (fun _       -> True)
         (fun h0 x h1 -> modifies (Set.singleton (addr_of r)) h0 h1 /\  //only modify the eref
 	             sel h0 r == sel h1 r                       /\  //value remains same
@@ -124,7 +129,7 @@ abstract let freeze (#a:Type0) (r:eref a{readable r})  //the precondition that w
 	             r `frozen_at` x)                              //and you get the stable predicate
   = admit ()
 
-abstract let recall_freeze (#a:Type0) (r:eref a) (x:a{r `frozen_at` x})
+let recall_freeze (#a:Type0) (r:eref a) (x:a{r `frozen_at` x})
   :ST unit (requires (fun _       -> True))
            (ensures  (fun h0 _ h1 -> h0 == h1 /\ sel h1 r == Some x))
   = admit ()
