sol/SwapIntRefsST.fst
@@ -9,28 +9,24 @@ val swap_add_sub : r1:ref int -> r2:ref int ->
                                     sel h3 r1 == sel h0 r2 /\
                                     sel h3 r2 == sel h0 r1))
 let swap_add_sub r1 r2 =
-  r1 := !r1 + !r2;
-  (*Know (P1) : exists h1. modifies !{r1} h0 h1
-                        /\ sel h1 r1 = (sel h0 r1) + (sel h0 r2) *)
-  r2 := !r1 - !r2;
-  (*Know (P2) : exists h2. modifies !{r2} h1 h2
-                        /\ sel h2 r2 = (sel h1 r1) - (sel h1 r2) *)
-  r1 := !r1 - !r2
-  (*Know (P3) :            modifies !{r1} h2 h3
-                        /\ sel h3 r1 = (sel h2 r1) - (sel h2 r2) *)
+  r1 := !r1 + !r2; (* Know (P1) : exists h1. modifies !{r1} h0 h1
+                               /\ sel h1 r1 = (sel h0 r1) + (sel h0 r2) *)
+  r2 := !r1 - !r2; (* Know (P2) : exists h2. modifies !{r2} h1 h2
+                               /\ sel h2 r2 = (sel h1 r1) - (sel h1 r2) *)
+  r1 := !r1 - !r2  (* Know (P3) :            modifies !{r1} h2 h3
+                               /\ sel h3 r1 = (sel h2 r1) - (sel h2 r2) *)
 
-  (* F* computed pre for this code is `fun _ -> True` *)
-  (* F* computed post for this code is `fun h0 _ h3 -> (P1) /\ (P2) /\ (P3)` *)
-  (* to show (1) : user-provided pre ==> F* computed pre (=True). Trivial. *)
-  (* - by additivity of modifies we get `modifies !{r1,r2} h0 h3` *)
-  (* to show (2): F* computed post /\ user-provided pre ==> user-provided post *)
-  (* - for instance, to show `sel h3 r1 == sel h0 r2` we reason as follows:
-          sel h3 r1 = (sel h2 r1) - (sel h2 r2)                    -- by (P3)
-                    = (sel h2 r1) - ((sel h1 r1) - (sel h1 r2))    -- by (P2)
-                    = sel h1 r2     -- by arithmetic and absence of underflows
-                    = sel h0 r2     -- by `addr_of r1 <> addr_of r2`
-                                       and `modifies !{r1} h0 h1`
-      *)
+(* F* computed pre for this code is `fun _ -> True` *)
+(* F* computed post for this code is `fun h0 _ h3 -> (P1) /\ (P2) /\ (P3)` *)
+(* to show (1) : user-provided pre ==> F* computed pre (=True). Trivial. *)
+(* - by additivity of modifies we get `modifies !{r1,r2} h0 h3` *)
+(* to show (2): F* computed post /\ user-provided pre ==> user-provided post *)
+(* - for instance, to show `sel h3 r1 == sel h0 r2` we reason as follows:
+        sel h3 r1 = (sel h2 r1) - (sel h2 r2)                    -- by (P3)
+                  = (sel h2 r1) - ((sel h1 r1) - (sel h1 r2))    -- by (P2)
+                  = sel h1 r2     -- by arithmetic and absence of underflows
+                  = sel h0 r2     -- by `modifies !{r1} h0 h1`
+                                     and `addr_of r1 <> addr_of r2`    *)
 // END: swap_add_sub
 
 open FStar.IO
